pulse/lib/steel/Steel.ST.GenArraySwap.fst
@@ -47,6 +47,8 @@ let gcd_post
 = SZ.v l0 < SZ.v n0 /\
   SZ.v res == (Prf.mk_bezout (SZ.v n0) (SZ.v l0)).d
 
+#push-options "--z3rlimit 16"
+
 #restart-solver
 let gcd
   (n0: SZ.t)
@@ -95,6 +97,8 @@ let gcd
   in
   elim_pure (gcd_post n0 l0 res);
   return res
+
+#pop-options
 
 let array_swap_partial_invariant
   (#t: Type)
@@ -167,24 +171,6 @@ let array_swap_outer_invariant_prop
   (b == (i < bz.d))
 
 #restart-solver
-let array_swap_outer_invariant_prop_begin
-  (#t: Type)
-  (n: nat)
-  (l: nat)
-  (bz: Prf.bezout n l)
-  (s0: Ghost.erased (Seq.seq t))
-: Lemma
-  (requires (
-    n == Seq.length s0 /\
-    0 < l /\
-    l < n
-  ))
-  (ensures (
-    array_swap_outer_invariant_prop n l bz s0 s0 0 true
-  ))
-= ()
-
-#restart-solver
 let array_swap_outer_invariant_prop_end
   (#t: Type)
   (n: nat)
@@ -193,13 +179,17 @@ let array_swap_outer_invariant_prop_end
   (s0: Ghost.erased (Seq.seq t))
   (s: Ghost.erased (Seq.seq t))
   (i: nat)
+  (b: bool)
 : Lemma
   (requires (
-    array_swap_outer_invariant_prop n l bz s0 s i false
+    array_swap_outer_invariant_prop n l bz s0 s i b /\
+    b == false
   ))
   (ensures (
+    array_swap_outer_invariant_prop n l bz s0 s i false /\
     Ghost.reveal s `Seq.equal` (Seq.slice s0 l n `Seq.append` Seq.slice s0 0 l)
   ))
+  [SMTPat (array_swap_outer_invariant_prop n l bz s0 s i b)]
 = Classical.forall_intro (Prf.jump_if n l ());
   let p
     (idx: Prf.nat_up_to n)
@@ -217,6 +207,26 @@ let array_swap_outer_invariant_prop_end
   Prf.jump_iter_elim n p l bz
 
 [@@__reduce__]
+let array_swap_outer_invariant_body0
+  (#t: Type)
+  (pts_to: array_pts_to_t t)
+  (pi: R.ref SZ.t)
+  (i: SZ.t)
+  (s: Ghost.erased (Seq.seq t))
+: Tot vprop
+=
+    R.pts_to pi full_perm i `star`
+    pts_to s
+
+[@@erasable]
+noeq
+type array_swap_outer_invariant_t (t: Type)
+= {
+    i: SZ.t;
+    s: Ghost.erased (Seq.seq t);
+  }
+
+[@@__reduce__]
 let array_swap_outer_invariant0
   (#t: Type)
   (pts_to: array_pts_to_t t)
@@ -227,11 +237,10 @@ let array_swap_outer_invariant0
   (pi: R.ref SZ.t)
   (b: bool)
 : Tot vprop
-= exists_ (fun i -> exists_ (fun s ->
-    R.pts_to pi full_perm i `star`
-    pts_to s `star`
-    pure (array_swap_outer_invariant_prop (SZ.v n) (SZ.v l) bz s0 s (SZ.v i) b)
-  ))
+= exists_ (fun w ->
+    array_swap_outer_invariant_body0 pts_to pi w.i w.s `star`
+    pure (array_swap_outer_invariant_prop (SZ.v n) (SZ.v l) bz s0 w.s (SZ.v w.i) b)
+ )
 
 let array_swap_outer_invariant
   (#t: Type)
@@ -244,6 +253,55 @@ let array_swap_outer_invariant
   (b: bool)
 : Tot vprop
 = array_swap_outer_invariant0 pts_to n l bz s0 pi b
+
+let intro_array_swap_outer_invariant
+  (#opened: _)
+  (#t: Type)
+  (pts_to: array_pts_to_t t)
+  (n: SZ.t)
+  (l: SZ.t)
+  (bz: Prf.bezout (SZ.v n) (SZ.v l))
+  (s0: Ghost.erased (Seq.seq t))
+  (pi: R.ref SZ.t)
+  (b: bool)
+  (i: SZ.t)
+  (s: Ghost.erased (Seq.seq t))
+: STGhost unit opened
+    (array_swap_outer_invariant_body0 pts_to pi i s)
+    (fun _ -> array_swap_outer_invariant pts_to n l bz s0 pi b)
+    (array_swap_outer_invariant_prop (SZ.v n) (SZ.v l) bz s0 s (SZ.v i) b)
+    (fun _ -> True)
+= let w = {
+    i = i;
+    s = s;
+  }
+  in
+  rewrite (array_swap_outer_invariant_body0 pts_to pi i s) (array_swap_outer_invariant_body0 pts_to pi w.i w.s);
+  rewrite (array_swap_outer_invariant0 pts_to n l bz s0 pi b) (array_swap_outer_invariant pts_to n l bz s0 pi b)
+
+let elim_array_swap_outer_invariant
+  (#opened: _)
+  (#t: Type)
+  (pts_to: array_pts_to_t t)
+  (n: SZ.t)
+  (l: SZ.t)
+  (bz: Prf.bezout (SZ.v n) (SZ.v l))
+  (s0: Ghost.erased (Seq.seq t))
+  (pi: R.ref SZ.t)
+  (b: bool)
+: STGhost (array_swap_outer_invariant_t t) opened
+    (array_swap_outer_invariant pts_to n l bz s0 pi b)
+    (fun w -> array_swap_outer_invariant_body0 pts_to pi w.i w.s)
+    True
+    (fun w ->
+      array_swap_outer_invariant_prop (SZ.v n) (SZ.v l) bz s0 w.s (SZ.v w.i) b /\
+True //      (b == false ==> Ghost.reveal w.s `Seq.equal` (Seq.slice s0 (SZ.v l) (SZ.v n) `Seq.append` Seq.slice s0 0 (SZ.v l)))
+    )
+= let w = elim_exists () in
+  let _ = gen_elim () in
+//  Classical.move_requires (array_swap_outer_invariant_prop_end (SZ.v n) (SZ.v l) bz s0 w.s (SZ.v w.i)) b;
+  noop ();
+  w
 
 [@@erasable]
 noeq
@@ -399,7 +457,7 @@ let array_swap_aux_post
       SZ.v l < SZ.v n /\
       Ghost.reveal s == Seq.slice s0 (SZ.v l) (SZ.v n) `Seq.append` Seq.slice s0 0 (SZ.v l)
 
-#push-options "--z3rlimit 64"
+#push-options "--z3rlimit 128"
 
 #restart-solver
 inline_for_extraction
@@ -424,7 +482,7 @@ let array_swap_outer_body
     (array_swap_outer_invariant pts_to n l bz s0 pi true)
     (fun _ -> exists_ (array_swap_outer_invariant pts_to n l bz s0 pi))
 =
-  rewrite (array_swap_outer_invariant pts_to n l bz s0 pi true) (array_swap_outer_invariant0 pts_to n l bz s0 pi true);
+  let _ = elim_array_swap_outer_invariant pts_to n l bz s0 pi true in
   let _ = gen_elim () in
   let i = R.read pi in
   let s = vpattern_replace pts_to in
@@ -460,13 +518,16 @@ let array_swap_outer_body
     let _ = elim_array_swap_inner_invariant pts_to n l bz s0 pi i pj pidx false in
     let idx = R.read pidx in
     let _ = upd _ n idx save in
-    Prf.jump_jump_iter_pred_q (SZ.v n) (SZ.v l) bz (SZ.v i);
     [@@inline_let]
     let i' = i `SZ.add` 1sz in
     R.write pi i';
-    rewrite (array_swap_outer_invariant0 pts_to n l bz s0 pi (i' `SZ.lt` d)) (array_swap_outer_invariant pts_to n l bz s0 pi (i' `SZ.lt` d));
+    intro_array_swap_outer_invariant pts_to n l bz s0 pi (i' `SZ.lt` d) _ _;
     noop ()
   ))
+
+#pop-options
+
+#push-options "--z3rlimit 128 --split_queries always" // WHY WHY WHY is the pattern on array_swap_outer_invariant_prop_end SO hard to trigger?
 
 #restart-solver
 inline_for_extraction
@@ -487,42 +548,28 @@ let array_swap_aux
       SZ.v l < SZ.v n
     )
     (fun s -> array_swap_aux_post s0 n l s)
-= let bz : Prf.bezout (SZ.v n) (SZ.v l) = Prf.mk_bezout (SZ.v n) (SZ.v l) in
+= let bz = Prf.mk_bezout (SZ.v n) (SZ.v l) in
   let d = gcd n l in
   let q = n `SZ.div` d in
-  assert (SZ.v d == bz.d);
-  FStar.Math.Lemmas.cancel_mul_div bz.q_n bz.d;
-  assert (SZ.v q == bz.q_n);
-  assert (SZ.v q > 0);
-  noop ();
   let s = R.with_local 0sz (fun pi ->
-    array_swap_outer_invariant_prop_begin (SZ.v n) (SZ.v l) bz s0;
-    noop ();
-    rewrite (array_swap_outer_invariant0 pts_to n l bz s0 pi true) (array_swap_outer_invariant pts_to n l bz s0 pi true);
+    intro_array_swap_outer_invariant pts_to n l bz s0 pi true _ _;
     Steel.ST.Loops.while_loop
       (array_swap_outer_invariant pts_to n l bz s0 pi)
       (fun _ ->
         let gb = elim_exists () in
-        rewrite (array_swap_outer_invariant pts_to n l bz s0 pi gb) (array_swap_outer_invariant0 pts_to n l bz s0 pi gb);
-        let _ = gen_elim () in
+        let _ = elim_array_swap_outer_invariant pts_to n l bz s0 pi gb in
         let i = R.read pi in
         [@@inline_let]
         let b = i `SZ.lt` d in
-        noop ();
-        rewrite (array_swap_outer_invariant0 pts_to n l bz s0 pi b) (array_swap_outer_invariant pts_to n l bz s0 pi b);
+        intro_array_swap_outer_invariant pts_to n l bz s0 pi b _ _;
         return b
       )
       (array_swap_outer_body index upd s0 n l bz d q pi ());
-    rewrite (array_swap_outer_invariant pts_to n l bz s0 pi false) (array_swap_outer_invariant0 pts_to n l bz s0 pi false);
-    let _ = gen_elim () in
-    let i = vpattern_erased (R.pts_to pi full_perm) in
-    let s = vpattern_replace pts_to in
-    array_swap_outer_invariant_prop_end (SZ.v n) (SZ.v l) bz s0 s (SZ.v i);
-    noop ();
-    return s
-  )
+    let _ = elim_array_swap_outer_invariant pts_to n l bz s0 pi false in
+    return _
+  ) <: STT (Ghost.erased (Seq.seq t)) _ (fun s -> pts_to s `star` pure (array_swap_aux_post s0 n l s))
   in
-  elim_pure (array_swap_aux_post s0 n l s);
+  elim_pure _;
   return s
 
 #pop-options
